attention has each kernel call

src/lib/kernel/Kuiper.Kernel.Attention.fst
@@ -7,16 +7,21 @@ open Kuiper.Tensor.Layout { ctlayout }
 open Kuiper.Tensor.Layout.Alg
 open Kuiper.Tensor
 open Kuiper.Index
+open Kuiper.EMatrix
 open Kuiper.Bijection
 
 module EM4 = Kuiper.EMatrix4
 module EM3 = Kuiper.EMatrix3
+module A2 = Kuiper.Array2
 module CH = Kuiper.Chest
 module SZ = Kuiper.SizeT
+module MS = Kuiper.Spec.GEMM
 
 open Kuiper.Spec.Attention
 open Kuiper.Kernel.BatchedGEMM
-
+open Kuiper.Kernel.RowSoftmax
+open Kuiper.Kernel.HReduce.Block
+open Kuiper.Kernel.Map
 
 #push-options "--split_queries always"
 let transpose4_2 (#d0 #d1 #d2 #d3 : nat) : 
@@ -35,7 +40,137 @@ let transpose4_2 (#d0 #d1 #d2 #d3 : nat) :
   ));
 }
 
+inline_for_extraction noextract
+fn fold4_to_3 
+  (#et : Type0) {| floating et, real_like et |}
+  (#d0 #d1 #d2 #d3: szp)
+  (#lA : tlayout (d0 @| d1 @| d2 @| d3 @| INil) { is_full lA })
+  {| ctlayout lA |}
+  (gA : tensor et lA { is_global gA })
+  (#fA : perm)
+  (#eA : erased (EM4.t et d0 d1 d2 d3))
+  (#rA : erased (EM4.t real d0 d1 d2 d3) { eA %~ rA })
+preserves
+  cpu
+requires
+  on gpu_loc (gA |-> Frac fA eA)
+returns
+  out : (
+    tensor et (tlayout_fold_outer lA <: tlayout ((d0 *^ d1) @| d2 @| d3 @| INil)) &
+    EM3.t et (d0 *^ d1) d2 d3 &
+    EM3.t real (d0 *^ d1) d2 d3 
+  ) 
+ensures 
+  on gpu_loc (out._1 |-> Frac fA (out._2)) **
+  pure (is_global out._1 /\ (out._2 %~ out._3) /\ out._3 == fold_chest rA)
+{
+  let gAf = from_array (tlayout_fold_outer lA) (core gA);
+  let eAf = fold_chest eA;
+  let rAf = fold_chest rA;
+  assert rewrites_to gAf (from_array (tlayout_fold_outer lA) (core gA));
+  map_loc gpu_loc (fun () -> tensor_fold_outer gA #fA);
+  return (gAf, eAf, rAf);
+}
+
+inline_for_extraction noextract
+fn fold3_to_2 
+  (#et : Type0) {| floating et, real_like et |}
+  (#d0 #d1 #d2: szp)
+  (#lA : tlayout (d0 @| d1 @| d2 @| INil) { is_full lA })
+  {| ctlayout lA |}
+  (gA : tensor et lA { is_global gA })
+  (#fA : perm)
+  (#eA : erased (EM3.t et d0 d1 d2))
+  (#rA : erased (EM3.t real d0 d1 d2) { eA %~ rA })
+preserves
+  cpu
+requires
+  on gpu_loc (gA |-> Frac fA eA)
+returns
+  out : (
+    tensor et (tlayout_fold_outer lA <: tlayout ((d0 *^ d1) @| d2 @| INil)) &
+    ematrix et (d0 *^ d1) d2 &
+    ematrix real (d0 *^ d1) d2 
+  ) 
+ensures 
+  on gpu_loc (out._1 |-> Frac fA (out._2)) **
+  pure (is_global out._1 /\ (out._2 %~ out._3) /\ out._3 == fold_chest rA)
+{
+  let gAf = from_array (tlayout_fold_outer lA) (core gA);
+  let eAf = fold_chest eA;
+  let rAf = fold_chest rA;
+  assert rewrites_to gAf (from_array (tlayout_fold_outer lA) (core gA));
+  map_loc gpu_loc (fun () -> tensor_fold_outer gA #fA);
+  return (gAf, eAf, rAf);
+}
+
+inline_for_extraction noextract
+fn unfold2_to_3 
+  (#et : Type0) {| floating et, real_like et |}
+  (#d0 #d1 #d2: szp)
+  (#lA : tlayout (d0 @| d1 @| d2 @| INil) { is_full lA })
+  {| ctlayout lA |}
+  (gA : tensor et (tlayout_fold_outer lA <: tlayout ((d0 *^ d1) @| d2 @| INil)) { is_global gA })
+  (#fA : perm)
+  (#eA : erased (ematrix et (d0 *^ d1) d2))
+  (#rA : erased (ematrix real (d0 *^ d1) d2) { eA %~ rA })
+preserves
+  cpu
+requires
+  on gpu_loc (gA |-> Frac fA eA)
+returns
+  out : (
+    tensor et lA &
+    EM3.t et d0 d1 d2 &
+    EM3.t real d0 d1 d2 
+  ) 
+ensures 
+  on gpu_loc (out._1 |-> Frac fA (out._2)) **
+  pure (is_global out._1 /\ (out._2 %~ out._3) /\ out._3 == unfold_chest rA)
+{
+  let gAuf = from_array lA (core gA);
+  let eAuf = unfold_chest #et #3 #(d0 @| d1 @| d2 @| INil) eA;
+  let rAuf = unfold_chest #real #3 #(d0 @| d1 @| d2 @| INil) rA;
+  assert rewrites_to gAuf (from_array lA (core gA));
+  map_loc gpu_loc (fun () -> tensor_unfold_outer gA #fA);
+  return (gAuf, eAuf, rAuf);
+}
+
+inline_for_extraction noextract
+fn fold4_to_2 
+  (#et : Type0) {| floating et, real_like et |}
+  (#d0 #d1 #d2 #d3: szp)
+  (#lA : tlayout (d0 @| d1 @| d2 @| d3 @| INil) { is_full lA })
+  {| ctlayout lA |}
+  (gA : tensor et lA { is_global gA })
+  (#fA : perm)
+  (#eA : erased (EM4.t et d0 d1 d2 d3))
+  (#rA : erased (EM4.t real d0 d1 d2 d3) { eA %~ rA })
+preserves
+  cpu
+requires
+  on gpu_loc (gA |-> Frac fA eA)
+returns
+  out : (
+    tensor et ((tlayout_fold_outer (tlayout_fold_outer lA)) <: tlayout ((d0 *^ d1 *^ d2) @| d3 @| INil)) &
+    ematrix et (d0 *^ d1 *^ d2) d3 &
+    ematrix real (d0 *^ d1 *^ d2) d3 
+  ) 
+ensures 
+  on gpu_loc (out._1 |-> Frac fA (out._2)) **
+  pure (is_global out._1 /\ (out._2 %~ out._3) /\ out._3 == fold_chest (fold_chest rA)) 
+{
+  let gAf,eAf,rAf = fold4_to_3 gA #fA #eA #rA;
+  let gAff = from_array (tlayout_fold_outer (tlayout_fold_outer lA)) (core gAf);
+  assert rewrites_to gAff (from_array (tlayout_fold_outer (tlayout_fold_outer lA)) (core gAf));
+  map_loc gpu_loc (fun () -> tensor_fold_outer gAf #fA);
+  let eAff = fold_chest eAf;
+  let rAff = fold_chest rAf;
+  return (gAff, eAff, rAff);
+}
+
 //#push-options "--print_implicits"
+inline_for_extraction noextract
 fn scaled_dot_product_efficient_attention
   (#et : Type0) {| floating et, real_like et, floating_real_like et |}
   (n h : szp)
@@ -69,11 +204,14 @@ fn scaled_dot_product_efficient_attention
       SZ.fits (n * h * l * e) /\
       SZ.fits (n * h * s * e)  /\
       SZ.fits (n * h * s * ev)  /\
+      SZ.fits (n * h * l * ev)  /\ 
       SZ.fits (n * h * l * s)  /\
       SZ.fits (n * h * l) /\
       (EM4.mkM (fun i j k l -> EM4.macc eK i j l k)) %~ rKT /\
       l * s <= max_blocks * max_threads /\
-      n * h * l <= max_blocks
+      l * ev <= max_blocks * max_threads /\
+      n * h * l <= max_blocks /\
+      n * h * l * s <= max_blocks * max_threads
     )
   returns
     // TODO: polymorphic out & LSE layout
@@ -100,7 +238,7 @@ fn scaled_dot_product_efficient_attention
   
   let rQ = EM4.to_real_matrix eQ;
   let rV = EM4.to_real_matrix eV;
-  let rbias = EM3.to_real_matrix ebias;
+  let rbias = EM4.to_real_matrix ebias;
 
   // Transpose K via ghost
   let f_transpose = transpose4_2 #n #h #s #e; 
@@ -111,35 +249,66 @@ fn scaled_dot_product_efficient_attention
   assert on gpu_loc (gKT |-> Frac fK eKT);
   assert pure (eKT %~ rKT);
 
-  // Fold 2 batch dimensions of K^T, Q, V into one (N * H)
-  let gKTf = from_array (tlayout_fold_outer (tlayout_bij f_transpose lK)) (core gKT);
-  let gQf = from_array (tlayout_fold_outer lQ) (core gQ);
-  let gVf = from_array (tlayout_fold_outer lV) (core gV);
-  let gbiasf = from_array (tlayout_fold_outer lbias) (core gbias);
-  assert rewrites_to gKTf (from_array (tlayout_fold_outer (tlayout_bij f_transpose lK)) (core gKT));
-  assert rewrites_to gQf (from_array (tlayout_fold_outer lQ) (core gQ));
-  assert rewrites_to gVf (from_array (tlayout_fold_outer lV) (core gV));
-  assert rewrites_to gbiasf (from_array (tlayout_fold_outer lbias) (core gbias));
-  
-  map_loc gpu_loc (fun () -> tensor_fold_outer gQ #fQ);
-  map_loc gpu_loc (fun () -> tensor_fold_outer gV #fV);
-  map_loc gpu_loc (fun () -> tensor_fold_outer gKT #fK);
-  map_loc gpu_loc (fun () -> tensor_fold_outer gbias #fbias);
+  // Fold 2 batch dimensions of K^T, Q, V, bias into one (N * H)
+  let gKTf, eKTf, rKTf = fold4_to_3 gKT #fK #eKT #rKT;
+  let gQf, eQf, rQf = fold4_to_3 gQ #fQ #eQ #rQ;
+  let gVf, eVf, rVf = fold4_to_3 gV #fV #eV #rV;
+  let gbiasf, ebiasf, rbiasf = fold4_to_3 gbias #fbias #ebias #rbias;
 
-  let eQf = fold_chest eQ; 
-  let eVf = fold_chest eV; 
-  let eKTf = fold_chest eKT; 
-  let ebiasf = fold_chest ebias;
-  assert on gpu_loc (gQf |-> Frac fQ eQf) ** pure (eQf %~ fold_chest rQ);
-  assert on gpu_loc (gVf |-> Frac fV eVf) ** pure (eVf %~ fold_chest rV);
-  assert on gpu_loc (gKTf |-> Frac fK eKTf) ** pure (eKTf %~ fold_chest rKT);
-  assert on gpu_loc (gbiasf |-> Frac fbias ebiasf) ** pure (ebiasf %~ fold_chest rbias);
-  
   let gS = alloc0 #et (n *^ h *^ l *^ s) (l3_batched_row_major (n*^h) l s);
   with eS. assert on gpu_loc (gS |-> eS);
 
-  bmmcomb_gpu_exact #et (fun bias_qk score -> (bias_qk +. score) *. scale) 
-    (n*^h) l e s gQf gKTf gS;
+  let lKT : tlayout (n @| h @| e @| s @| INil) = tlayout_bij f_transpose lK;
+  let ctlKT : ctlayout lKT = ctlayout_bij f_transpose lK;
+  bmmcomb_gpu_exact #et (fun bias_qk score -> (bias_qk `add` score) `mul` scale) 
+    (n*^h) l e s #_ #_ #_ #(ctlayout_bij fold_bij lQ) #(ctlayout_bij fold_bij lKT) #_ gQf gKTf gS;
+  with eS'. assert on gpu_loc (gS |-> (eS' <: EM3.t et (n *^ h) l s));
 
-  admit ();
+  let rS': EM3.t real (n *^ h) l s = MS.bmmcomb 
+    (fun bias_qk score -> (bias_qk +. score) *. (to_real scale))
+    rbiasf rQf rKTf;
+  assume pure ((eS' <: EM3.t et (n *^ h) l s) %~ rS'); // TODO
+
+  let gSf, eSf, rSf = fold3_to_2 gS #_ #eS' #rS';
+
+  // TODO: could fuse some `f` with the sums in this kernel, for the log step
+  let sums = row_softmax_gpu_with_sum (n *^ h *^ l) s 
+    #(tlayout_fold_outer (l3_batched_row_major (n*^h) l s))
+    #(ctlayout_bij fold_bij (l3_batched_row_major (n*^h) l s))
+    gSf rSf;
+  with esums. assert on gpu_loc (sums |-> esums);
+  assert pure (esums %~ Seq.init_ghost (n *^ h *^ l) (fun i -> rsum (lseq_map exp (ematrix_row rSf i))));
+  map_gpu flog (n *^ h *^ l) sums;
+  with esums'. assert on gpu_loc (sums |-> esums');
+  assert pure (esums' == lseq_map flog esums);
+  // causes z3 assertion violation (just typechecking the proposition, not proving it).. TODO
+  // assume pure (
+  //   ((Seq.init_ghost #real (n *^ h *^ l) (fun i -> log (rsum (lseq_map exp (ematrix_row rSf i))))) <: lseq real (n *^ h *^ l)) 
+  //   == 
+  //   lseq_map #real #real log (Seq.init_ghost #(r: real {r >. 0.0R}) (n *^ h *^ l) (fun i -> 
+  //     rsum (lseq_map exp (ematrix_row rSf i)) <: (r: real {r >. 0.0R}))));
+  assume pure (esums' %~ Seq.init_ghost (n *^ h *^ l) (fun i -> log (rsum (lseq_map exp (ematrix_row rSf i))))); // TODO
+
+  with eSf. assert on gpu_loc (gSf |-> eSf);
+  let eSf: ematrix et (n *^ h *^ l) s = eSf;
+  assert pure (eSf %~ row_softmax_real rSf);
+  let gS, eS, rS = unfold2_to_3 gSf #_ #eSf #(row_softmax_real rSf);
+
+  let gO = alloc0 #et (n *^ h *^ l *^ ev) (l3_batched_row_major (n*^h) l ev);
+  with eO. assert on gpu_loc (gO |-> eO);
+
+  bmmcomb_gpu_exact #et MS.comb2 
+    (n*^h) l s ev #_ #_ #_ #_ #(ctlayout_bij fold_bij lV) #_ gS gVf gO;
+
+(*
+  complete the proof/function; rough steps:
+  1. add an unfold3_to_4 function that lets us convert gKTf, gQf, gVf, gbiasf back to their original 4D shapes (and prove that the unfolded versions are equivalent to the original tensors)
+  2. do the same for gO, and prove the functional specification (attention_real)
+      - this is conceptually simple because we just need to show that basically doing these operations on 3d matrices is the same as 
+        doing them on 2D matrices and then creating a 4D matrix with chest.mk as in the spec.
+  3. turn the flattened LSE array1 into a 3D tensor and show it approximtes the spec. 
+      raise/lower in Array1 should be helpful for this. you probably want to make it into a separate lemma (array1_to_3d or something.)
+  4. free sums.
+*)
+  admit ()
 }
